On the way of improving local2ptree. But not finish.

floyd/local2ptree.v
@@ -13,42 +13,80 @@ Require Import floyd.efield_lemmas.
 Local Open Scope logic.
 
 Inductive local2ptree:
-  list (environ -> Prop) -> PTree.t val -> PTree.t (type * val) -> list (environ -> Prop) -> Prop :=
+  list (environ -> Prop) -> PTree.t val -> PTree.t (type * val)
+    -> list Prop -> list (environ -> Prop) -> Prop :=
   | local2ptree_nil:
-      local2ptree nil (PTree.empty _) (PTree.empty _) nil
-  | local2ptree_temp_var: forall v i Q T1 T2 Q',
-      local2ptree Q T1 T2 Q'->
-      local2ptree (temp i v :: Q) (PTree.set i v T1) T2 Q'
-  | local2ptree_gl_var: forall v i t Q T1 T2 Q',
-      local2ptree Q T1 T2 Q'->
-      local2ptree (var i t v :: Q) T1 (PTree.set i (t, v) T2) Q'
-  | local2ptree_unknown: forall Q0 Q T1 T2 Q',
-      local2ptree Q T1 T2 Q'->
-      local2ptree (Q0 :: Q) T1 T2 (Q0 :: Q').
+      local2ptree nil (PTree.empty _) (PTree.empty _) nil nil
+  | local2ptree_temp_var_first: forall v i Q T1 T2 P' Q',
+      local2ptree Q T1 T2 P' Q' ->
+      T1 ! i = None ->
+      local2ptree (temp i v :: Q) (PTree.set i v T1) T2 P' Q'
+  | local2ptree_temp_var_second: forall v v' i Q T1 T2 P' Q',
+      local2ptree Q T1 T2 P' Q' ->
+      T1 ! i = Some v' ->
+      local2ptree (temp i v :: Q) T1 T2 ((v = v') :: P') Q'
+  | local2ptree_gl_var_first: forall v i t Q T1 T2 P' Q',
+      local2ptree Q T1 T2 P' Q' ->
+      T2 ! i = None ->
+      local2ptree (var i t v :: Q) T1 (PTree.set i (t, v) T2) P' Q'
+  | local2ptree_gl_var_second: forall v v' i t Q T1 T2 P' Q',
+      local2ptree Q T1 T2 P' Q' ->
+      T2 ! i = Some (t, v') ->
+      local2ptree (var i t v :: Q) T1 T2 ((v = v') :: P') Q'
+  | local2ptree_unknown: forall Q0 Q T1 T2 P' Q',
+      local2ptree Q T1 T2 P' Q'->
+      local2ptree (Q0 :: Q) T1 T2 P' (Q0 :: Q').
 (* repeat constructor will try the first succesful tactic. So local2ptree_temp_ *)
 (* var, local2ptree_gl_var will be used whenever is possible before local2ptree_*)
 (* unknown.                                                                     *)
 
 Module TEST.
-Goal False.
-evar (T1: PTree.t val).
-evar (T2: PTree.t (type * val)).
-evar (Q' : list (environ -> Prop)).
 
-assert (local2ptree  ((`(eq Vundef) (eval_id 1%positive)) :: (`(eq (Vint (Int.repr 1))) (eval_id 1%positive)) :: 
-   (`(eq 1 3)) :: nil)
-  T1 T2 Q').
-subst T1 T2 Q'.
-repeat constructor; repeat simpl; auto.
-Abort.
+Ltac construct_local2ptree Q H :=
+  let T1 := fresh "T" in evar (T1: PTree.t val);
+  let T2 := fresh "T" in evar (T2: PTree.t (type * val));
+  let P' := fresh "P'" in evar (P' : list Prop);
+  let Q' := fresh "Q'" in evar (Q' : list (environ -> Prop));
+  assert (local2ptree Q T1 T2 P' Q') as H; [
+    subst T1 T2 P' Q';
+    match Q with
+    | @nil _ => exact local2ptree_nil
+    | (`(eq ?v) (eval_id ?i)) :: ?Q0 =>
+        let H0 := fresh "H" in
+        construct_local2ptree Q0 H0;
+        first [
+          eapply local2ptree_temp_var_first; [exact H0 | reflexivity] |
+          eapply local2ptree_temp_var_second; [exact H0 | reflexivity]]
+    | (temp ?i ?v) :: ?Q0 =>
+        let H0 := fresh "H" in
+        construct_local2ptree Q0 H0;
+        first [
+          eapply local2ptree_temp_var_first; [exact H0 | reflexivity] |
+          eapply local2ptree_temp_var_second; [exact H0 | reflexivity]]
+    | (`(eq ?v) (eval_var ?i ?t)) :: ?Q0 =>
+        let H0 := fresh "H" in
+        construct_local2ptree Q0 H0;
+        first [
+          eapply local2ptree_gl_var_first; [exact H0 | reflexivity] |
+          eapply local2ptree_gl_var_second; [exact H0 | reflexivity] |
+          eapply local2ptree_unknown; exact H0]
+    | (var ?i ?t ?v) :: ?Q0 =>
+        let H0 := fresh "H" in
+        construct_local2ptree Q0 H0;
+        first [
+          eapply local2ptree_gl_var_first; [exact H0 | reflexivity] |
+          eapply local2ptree_gl_var_second; [exact H0 | reflexivity] |
+          eapply local2ptree_unknown; exact H0]
+    | ?QQ :: ?Q0 =>
+        let H0 := fresh "H" in
+        construct_local2ptree Q0 H0;
+        eapply local2ptree_unknown; exact H0
+    end|];
+  subst T1 T2 P' Q'.
 
 Goal False.
-evar (T1: PTree.t val).
-evar (T2: PTree.t (type * val)).
-evar (Q' : list (environ -> Prop)).
-assert (local2ptree ((`(eq Vundef) (eval_id 1%positive))::nil) T1 T2 Q').
-subst T1 T2 Q'.
-repeat constructor; repeat simpl; auto.
+  construct_local2ptree ((temp 1%positive Vundef) :: (`(eq (Vint (Int.repr 1))) (eval_id 1%positive)) :: 
+   (`(eq 1 3)) :: nil) H.
 Abort.
 End TEST.
 
@@ -250,65 +288,95 @@ Proof.
 Qed.
 
 Lemma LOCALx_expand_temp_var: forall i v T1 T2 Q Q0,
-  In Q0 (LocalD (PTree.set i v T1) T2 Q) -> 
-  In Q0 (temp i v :: LocalD T1 T2 Q).
+  In Q0 (LocalD (PTree.set i v T1) T2 Q) <-> 
+  In Q0 (temp i v :: LocalD (PTree.remove i T1) T2 Q).
 Proof.
-  intros.
-  simpl.
-  apply LocalD_complete in H.
-  destruct H.
-  + destruct H as [i0 [v0 [? ?]]].
-    destruct (ident_eq i0 i).
-    - subst.
-      rewrite PTree.gss in H.
-      inversion H; subst.
-      left; reflexivity.
-    - rewrite PTree.gso in H by auto.
-      right.
+  intros; split; intros.
+  + simpl.
+    apply LocalD_complete in H.
+    destruct H.
+    - destruct H as [i0 [v0 [? ?]]].
+      subst.
+      destruct (ident_eq i0 i).
+      * subst.
+        rewrite PTree.gss in H.
+        inversion H; subst.
+        left; reflexivity.
+      * rewrite PTree.gso in H by auto.
+        right.
+        apply LocalD_sound.
+        left.
+        exists i0, v0.
+        rewrite PTree.gro by auto.
+        split; [exact H | reflexivity].
+    - right.
       apply LocalD_sound.
-      left.
-      exists i0, v0.
-      exact (conj H H0).
-  + right.
-    apply LocalD_sound.
-    right.
-    exact H.
+      right.
+      exact H.
+  + simpl in H.
+    destruct H; subst; apply LocalD_sound.
+    - left.
+      exists i, v.
+      split; [apply PTree.gss | reflexivity].
+    - apply LocalD_complete in H.
+      destruct H.
+      * left.
+        destruct H as [i0 [v0 [? ?]]].
+        destruct (ident_eq i i0).
+        {
+          subst.
+          rewrite PTree.grs in H.
+          inversion H.
+        }
+        {
+          exists i0, v0.
+          rewrite PTree.gso by auto.
+          rewrite PTree.gro in H by auto.
+          split; [exact H | exact H0].
+        }
+      * right.
+        auto.
 Qed.
 
 Lemma LOCALx_expand_gl_var: forall i t v T1 T2 Q Q0,
-  In Q0 (LocalD T1 (PTree.set i (t, v) T2) Q) -> 
-  In Q0 (var i t v :: LocalD T1 T2 Q).
+  In Q0 (LocalD T1 (PTree.set i (t, v) T2) Q) <-> 
+  In Q0 (var i t v :: LocalD (PTree.remove i T1) T2 Q).
 Proof.
-  intros.
-  simpl.
-  apply LocalD_complete in H.
-  destruct H as [ |[ |]].
-  + right.
-    apply LocalD_sound.
-    left.
-    exact H.
-  + destruct H as [i0 [t0 [v0 [? ?]]]].
-    destruct (ident_eq i0 i).
-    - subst.
-      rewrite PTree.gss in H.
-      inversion H; subst.
-      left; reflexivity.
-    - rewrite PTree.gso in H by auto.
-      right.
+Admitted.
+(*
+  intros; split; intros.
+  + simpl.
+    apply LocalD_complete in H.
+    destruct H as [ |[ |]].
+    - right.
       apply LocalD_sound.
-      right; left.
-      exists i0, t0, v0.
-      exact (conj H H0).
-  + right.
-    apply LocalD_sound.
-    right; right.
-    exact H.
+      left.
+      exact H.
+    - destruct H as [i0 [t0 [v0 [? ?]]]].
+      destruct (ident_eq i0 i).
+      - subst.
+        rewrite PTree.gss in H.
+        inversion H; subst.
+        left; reflexivity.
+      - rewrite PTree.gso in H by auto.
+        right.
+        apply LocalD_sound.
+        right; left.
+        exists i0, t0, v0.
+        exact (conj H H0).
+    + right.
+      apply LocalD_sound.
+      right; right.
+      exact H.
 Qed.
+*)
 
 Lemma LOCALx_expand_res: forall Q1 T1 T2 Q Q0,
-  In Q0 (LocalD T1 T2 (Q1 ::Q)) -> 
+  In Q0 (LocalD T1 T2 (Q1 ::Q)) <-> 
   In Q0 (Q1 ::LocalD T1 T2 Q).
 Proof.
+Admitted.
+(*
   intros.
   simpl.
   apply LocalD_complete in H.
@@ -325,6 +393,7 @@ Proof.
       apply LocalD_sound.
       right; right; exact H.
 Qed.
+*)
 
 Lemma LOCALx_shuffle: forall P Q Q' R,
   (forall Q0, In Q0 Q' -> In Q0 Q) ->
@@ -440,6 +509,35 @@ Proof.
   apply LOCALx_expand_temp_var' in H.
   destruct H; [left; auto | right].
   apply LocalD_subst, H.
+Qed.
+
+Lemma local2ptree_soundness: forall P Q R T1 T2 P' Q',
+  local2ptree Q T1 T2 P' Q' ->
+  PROPx P (LOCALx Q (SEPx R)) = PROPx (P' ++ P) (LOCALx (LocalD T1 T2 Q') (SEPx R)).
+Proof.
+  intros.
+  induction H.
+  + unfold LocalD.
+    rewrite !PTree.fold_spec.
+    simpl.
+    reflexivity.
+  + rewrite <- insert_local.
+    rewrite IHlocal2ptree.
+    rewrite insert_local.
+    apply pred_ext; apply LOCALx_shuffle; intros.
+    - apply LOCALx_expand_temp_var; auto.
+    - Check LOCALx_expand_temp_var.
+SearchAbout temp.
+  + eapply derives_trans.
+    - rewrite <- insert_local.
+      apply andp_derives; [apply derives_refl | exact IHlocal2ptree].
+    - rewrite insert_local.
+      apply LOCALx_shuffle, LOCALx_expand_gl_var.
+  + eapply derives_trans.
+    - rewrite <- insert_local.
+      apply andp_derives; [apply derives_refl | exact IHlocal2ptree].
+    - rewrite insert_local.
+      apply LOCALx_shuffle, LOCALx_expand_res.
 Qed.
 
 Lemma local2ptree_soundness: forall P Q R T1 T2 Q',
